updates

Veritas.Verifier.EAC.fst
@@ -675,98 +675,94 @@ let lemma_non_eac_evicted_blum_addm
       hash_collision_contra()
   )
 
-(*
-
-let lemma_non_eac_evicted_merkle_addb (#p:pos)
-  (itsl: non_eac_ts_log p{
-    VG.hash_verifiable (partition_idx_seq itsl) /\
-    EACEvictedMerkle? (last_valid_eac_state itsl)  /\
-    AddB? (to_vlog_entry (invalidating_log_entry itsl))
+let lemma_non_eac_evicted_merkle_addb
+  (itsl: neac_log {
+    TL.hash_verifiable itsl /\  
+    EACEvictedMerkle? (eac_boundary_state_pre itsl) /\
+    AddB? (eac_boundary_entry itsl)
    })
   : hash_collision_gen =
-  (* hash verifiable - evict hash and add hash equal *)
-  let gl = partition_idx_seq itsl in
-  assert(VG.hadd gl = VG.hevict gl);
+  let gl = g_vlog_of itsl in  
+  let st = eac_boundary_state_pre itsl in
 
-  let st = last_valid_eac_state itsl in
-  let ee = invalidating_log_entry itsl in
-  assert(eac_add ee st = EACFail);
+  (* the maximum eac prefix of itsl *)
+  let i = eac_boundary itsl in
+  let itsli = I.prefix itsl i in
+  let itsli' = I.prefix itsl (i + 1) in
+
+  // vlog entry e going at thread tid causes the eac failure
+  let e = I.index itsl i in
+  let k = V.key_of e in
+  let tid = thread_id_of itsl i in
+  let ee = TL.vlog_entry_ext_at itsl i in
+
   match st with
-  | EACEvictedMerkle v_e -> (
+  | EACEvictedMerkle v_e  -> (
     match ee with
     | NEvict (AddB (k,v) t j) ->
-      let tsle = time_seq_ext itsl in
-      let i = max_eac_prefix tsle in
-      let (e,tid) = index itsl i in
-
-      let itsli = prefix itsl i in
-      (* verifier thread state of tid after itsli *)
-      let vsi = verifier_thread_state itsli tid in
-
-      let itsli' = prefix itsl (i + 1) in
-      let vsi' = verifier_thread_state itsli' tid in
-      lemma_verifier_thread_state_extend itsli';
-      assert(vsi' == t_verify_step vsi e);
 
       (* number of blum evicts is the same as blum adds in the first i entries *)
       lemma_evict_add_count_same_evictedm itsli k;
-      assert(MS.size (ts_add_set_key itsli k) = MS.size (ts_evict_set_key itsli k));
+      // assert(MS.size (ts_add_set_key itsli k) = MS.size (ts_evict_set_key itsli k));
 
       (* the ith element is a blum add *)
-      assert(is_blum_add #p (e,tid));
+      // assert(is_blum_add e);
+      assert(I.index itsl i = I.index itsli' i);
       lemma_ts_add_set_key_extend itsli';
-      assert(ts_add_set_key itsli' k == add_elem (ts_add_set_key itsli k)
-                                                 (blum_add_elem #p (e,tid)));
+      // assert(ts_add_set_key itsli' k == add_elem (ts_add_set_key itsli k) (blum_add_elem e));
 
       (* the ith element is not a blum evict *)
-      assert(not (is_blum_evict (index itsl i)));
+      // assert(not (is_evict_to_blum (I.index itsl i)));
       lemma_ts_evict_set_key_extend2 itsli';
-      assert(ts_evict_set_key itsli' k == ts_evict_set_key itsli k);
+      // assert(ts_evict_set_key itsli' k == ts_evict_set_key itsli k);
 
       (* this implies that the size of the add set after processing (i+1) elements
-         * is one larger than the evict set at this point *)
-      assert(MS.size (ts_add_set_key itsli' k) = 1 + (MS.size (ts_evict_set_key itsli' k)));
+       * is one larger than the evict set at this point *)
+      // assert(MS.size (ts_add_set_key itsli' k) = 1 + (MS.size (ts_evict_set_key itsli' k)));
 
       (* this implies that in the first (i+1) entries there is an element whose membership in
          * add multiset is > its membership in evict multiset *)
       let be = diff_elem (ts_add_set_key itsli' k) (ts_evict_set_key itsli' k) in
       lemma_ts_add_set_key_contains_only itsli' k be;
-      assert(MH.key_of be = k);
+      // assert(MH.key_of be = k);
 
       lemma_mem_key_add_set_same itsli' be;
       lemma_mem_key_evict_set_same itsli' be;
-      assert(MS.mem be (ts_add_set itsli') > MS.mem be (ts_evict_set itsli'));
+      // assert(MS.mem be (ts_add_set itsli') > MS.mem be (ts_evict_set itsli'));
 
       (* the index of be in the add set *)
       let i_be = some_add_elem_idx itsli' be in
-      assert(i_be <= i);
+      // assert(i_be <= i);
 
       (* from clock orderedness any evict_set entry for be should happen before i *)
       lemma_evict_before_add2 itsl i_be;
-      assert(MS.mem be (ts_evict_set itsl) = MS.mem be (ts_evict_set (prefix itsl i_be)));
+      // assert(MS.mem be (ts_evict_set itsl) = MS.mem be (ts_evict_set (I.prefix itsl i_be)));
 
       (* any set membership is monotonic *)
       lemma_mem_monotonic be itsl (i + 1);
       lemma_mem_monotonic be itsli' i_be;
-      assert(MS.mem be (ts_add_set itsl) >= MS.mem be (ts_add_set itsli'));
-      assert(MS.mem be (ts_evict_set itsl) = MS.mem be (ts_evict_set itsli'));
+      // assert(MS.mem be (ts_add_set itsl) >= MS.mem be (ts_add_set itsli'));
+      // assert(MS.mem be (ts_evict_set itsl) = MS.mem be (ts_evict_set itsli'));
 
       (* this implies the membership of be in (overall) addset > membership in evict set *)
       (* so these two sets are not equal providing a hash collision *)
-      assert(MS.mem be (ts_add_set itsl) > MS.mem be (ts_evict_set itsl));
+      // assert(MS.mem be (ts_add_set itsl) > MS.mem be (ts_evict_set itsl));
 
       MS.lemma_not_equal (ts_add_set itsl) (ts_evict_set itsl) be;
-      assert(~( (ts_add_set itsl) == (ts_evict_set itsl)));
+      // assert(~( (ts_add_set itsl) == (ts_evict_set itsl)));
 
       lemma_ts_add_set_correct itsl;
       lemma_ts_evict_set_correct itsl;
-      assert(~ (g_add_set gl == g_evict_set gl));
+      // assert(~ (g_add_set gl == g_evict_set gl));
 
       lemma_g_hadd_correct gl;
       lemma_ghevict_correct gl;
 
       MultiHashCollision (MSCollision (g_add_seq gl) (g_evict_seq gl))
   )
+
+
+(*
 
 let lemma_non_eac_evicted_blum_addb (#p:pos)
   (itsl: non_eac_ts_log p{
@@ -904,10 +900,10 @@ let lemma_non_eac_time_seq_implies_hash_collision
       | NEvict (Get _ _) -> lemma_non_eac_evicted_requires_key_in_store itsl
       | NEvict (Put _ _) -> lemma_non_eac_evicted_requires_key_in_store itsl      
       | NEvict (AddM (k,v) _) -> lemma_non_eac_evicted_merkle_addm itsl      
+      | NEvict (AddB _ _ _) ->  lemma_non_eac_evicted_merkle_addb itsl      
       | EvictMerkle (EvictM _ _) _ -> lemma_non_eac_evicted_requires_key_in_store itsl
       | EvictBlum (EvictB _ _) _ _ -> lemma_non_eac_evicted_requires_key_in_store itsl   
       | EvictBlum (EvictBM _ _ _) _ _ -> lemma_non_eac_evicted_requires_key_in_store itsl      
-      | _ -> admit()
     )
   | EACEvictedBlum v t tid -> (
     match ee with
@@ -917,8 +913,7 @@ let lemma_non_eac_time_seq_implies_hash_collision
       | EvictMerkle (EvictM _ _) _ -> lemma_non_eac_evicted_requires_key_in_store itsl
       | EvictBlum (EvictB _ _) _ _ -> lemma_non_eac_evicted_requires_key_in_store itsl   
       | EvictBlum (EvictBM _ _ _) _ _ -> lemma_non_eac_evicted_requires_key_in_store itsl      
-
-    | _ -> admit()
+      | _ -> admit()
     )
     
 
